FloatModel/Float/Basic.lean
@@ -13,10 +13,23 @@ public import FloatModel.Sign
 
 namespace FloatModel
 
+/--
+An inductive type representing a floating-point number with constructors for signed infinity,
+not-a-number without payload, signed zero, and finite floats with a sign, positive natural
+mantissa and integral exponent.
+
+Note that finite floats do not have a unique representation in this format: multiplying the
+mantissa by two and decreasing the exponent by one yields a finite float that represents the
+same rational number.
+-/
 inductive UnpackedFloat where
+  /-- Signed infinity. -/
   | infinity (sign : Sign) : UnpackedFloat
+  /-- Not a number. There is no payload attached to a NaN in this format. -/
   | notANumber : UnpackedFloat
+  /-- Signed zero. -/
   | zero (sign : Sign) : UnpackedFloat
+  /-- Finite floats consisting of a sign bit, a positive natural mantissa and an exponent. -/
   | finite (sign : Sign) (mantissa : Nat) (exponent : Int) (mantissa_pos : 0 < mantissa) : UnpackedFloat
 deriving Repr, BEq
 
