FloatModel/Float/Lemmas.lean
@@ -1,0 +1,35 @@
+/-
+Copyright (c) 2026 Lean FRO, LLC. All rights reserved.
+Released under Apache 2.0 license as described in the file LICENSE.
+Authors: Julia M. Himmel
+-/
+module
+
+public import FloatModel.Float.Valid
+public import FloatModel.Float.Round
+
+namespace FloatModel
+
+@[simp]
+theorem snd_shiftToTargetExponent {spec : FloatSpec} {mantissa : Nat} {exponent : Int}
+    {accuracy : Accuracy} :
+    (shiftToTargetExponent spec mantissa exponent accuracy).2 = max exponent (spec.targetExponent (totalExponent mantissa exponent)) := by
+  grind [shiftToTargetExponent]
+
+theorem totalExponent_shiftToTargetExponent {spec : FloatSpec} {mantissa : Nat} {exponent : Int}
+    {accuracy : Accuracy} :
+    totalExponent (shiftToTargetExponent spec mantissa exponent accuracy).1.mantissa (shiftToTargetExponent spec mantissa exponent accuracy).2 =
+    totalExponent mantissa exponent := by
+  sorry
+
+theorem valid_roundWithAccuracy {spec : FloatSpec} {sign : Sign} {mantissa : Nat} {exponent : Int}
+    {accuracy : Accuracy} (h : exponent ≤ spec.targetExponent (totalExponent mantissa exponent)) :
+    spec.Valid (roundWithAccuracy spec sign mantissa exponent accuracy) := by
+  fun_cases roundWithAccuracy with
+  | case1 => simp
+  | case2 em₁ e₁ hshift roundedEm₁ finalExtendedMantissa finalExponent hshift' finalMantissa hne =>
+    refine .finite _ _ _ _ ⟨?_, ?_⟩
+    · sorry
+    · sorry
+
+end FloatModel
