FloatModel/Float/Model.lean
@@ -1,0 +1,33 @@
+/-
+Copyright (c) 2026 Lean FRO, LLC. All rights reserved.
+Released under Apache 2.0 license as described in the file LICENSE.
+Authors: Julia M. Himmel
+-/
+module
+
+public import FloatModel.Float.Valid
+
+-- This file is part of the logical model for floats which authors of float libraries
+-- need to rely on.
+@[expose] public section
+
+namespace FloatModel
+
+/-- The type of unpacked floats that are in the specified format. -/
+structure ModelFloat (spec : FloatSpec) where
+  /-- The underlying unpacked float. -/
+  unpackedFloat : UnpackedFloat
+  /-- The unpacked float is valid according to the specification. -/
+  valid : spec.Valid unpackedFloat
+
+/-- The logical model for the `Float` type. -/
+structure Float.Model where
+  /-- The logical model of the float. -/
+  modelFloat : ModelFloat FloatSpec.binary64
+
+/-- The logical model for the `Float32` type. -/
+structure Float32.Model where
+  /-- The logical model of the float. -/
+  modelFloat : ModelFloat FloatSpec.binary32
+
+end FloatModel
