FloatModel/Float/Operations/Div.lean
@@ -35,7 +35,7 @@ def divCore (spec : FloatSpec) (m₁ : Nat) (e₁ : Int) (m₂ : Nat) (e₂ : In
   -- Strategy: decrease the exponent here far enough so that we definitely get enough bits in the
   -- quotient `m / m₂`. We take the `min` because we don't want to increase the exponent; this happens
   -- later in the rounding step.
-  let targetExponent := min (e₁ - e₂) (spec.targetExponent (m₁.log2 + 1 + e₁ - (m₂.log2 + 1 + e₂)))
+  let targetExponent := min (e₁ - e₂) (spec.targetExponent (totalExponent m₁ e₁ - totalExponent m₂ e₂))
   let shiftAmount := (e₁ - e₂ - targetExponent).toNat
   let m := m₁ <<< shiftAmount
   (m / m₂, targetExponent, accuracyOfFraction m₂ (m % m₂))
