FloatModel/Float/Valid.lean
@@ -1,0 +1,44 @@
+/-
+Copyright (c) 2026 Lean FRO, LLC. All rights reserved.
+Released under Apache 2.0 license as described in the file LICENSE.
+Authors: Julia M. Himmel
+-/
+module
+
+public import FloatModel.Float.Basic
+public import FloatModel.Float.FloatSpec
+
+-- This file is part of the logical model for floats which authors of float libraries
+-- need to rely on.
+@[expose] public section
+
+namespace FloatModel
+
+/--
+Predicate asserting that a `(mantissa, exponent)` pair has the correct format for the given
+`FloatSpec`.
+-/
+structure FloatSpec.ValidMantissaExponent (spec : FloatSpec) (mantissa : Nat) (exponent : Int) : Prop where
+  /--
+  The exponent has the correct exponent for the total exponent of the `(mantissa, exponent)` pair.
+  This ensures that the mantissa always takes the right number of bits, depending on whether the
+  number is normal or subnormal.
+  -/
+  eq_targetExponent : exponent = spec.targetExponent (totalExponent mantissa exponent)
+  /--
+  The exponent does not overflow the available bits.
+  -/
+  le_sub : exponent ≤ spec.infinityExponent - spec.mantissaBits
+
+/--
+Predicate asserting that an `UnpackedFloat` is in the correct format for the given `FloatSpec`.
+-/
+inductive FloatSpec.Valid (spec : FloatSpec) : UnpackedFloat → Prop where
+  | infinity s : Valid spec (.infinity s)
+  | notANumber : Valid spec .notANumber
+  | zero s : Valid spec (.zero s)
+  | finite s m e hm : spec.ValidMantissaExponent m e → Valid spec (.finite s m e hm)
+
+attribute [simp] FloatSpec.Valid.infinity FloatSpec.Valid.notANumber FloatSpec.Valid.zero
+
+end FloatModel
